used ndaStep lemma to proof medGeneral step

automat/CaseStudy/medGeneralAut.thy
@@ -1,6 +1,6 @@
 theory medGeneralAut
 
-imports PreludeMed
+imports PreludeMed automat.ndaTotal
 
 begin
 
@@ -12,14 +12,14 @@ fun medGeneralTransitionH :: "nat set \<Rightarrow> ('a \<Rightarrow> ('a tsyn s
 "medGeneralTransitionH _ dropBehaviour (Suc n) (Msg m) = { (  n  ,   out  ) | out . out\<in>(dropBehaviour m)   }" |  (* Drop *)
 "medGeneralTransitionH resetSet  _        0    (Msg m) = { (  n  , (Msg m)) | n. n \<in> resetSet}"     (* Pass *)
 
-fun tsynDelay :: "nat \<Rightarrow> 'm tsyn SB \<Rightarrow> 'm tsyn SB" where
-"tsynDelay n tsb = undefined" (* ToDo: Should be -- ubConcEq (sbNTimes n (tsynNull (ubDom tsb))) tsb *)
+definition tsynDelay :: "nat \<Rightarrow> 'm::message tsyn SB \<rightarrow> 'm tsyn SB" where
+"tsynDelay n = ubConcEq (sbNTimes n (tsynbNull  (\<C> ''in'')))" 
 
 (* ToDo: use delaySet to nondeterministically delay everything *)
 fun medGeneralTransition :: "nat set \<Rightarrow> medState set \<Rightarrow> ('a \<Rightarrow> ('a tsyn set)) \<Rightarrow> (medState \<times> 'a medMessage tsyn sbElem) \<Rightarrow> ((medState \<times> 'a medMessage tsyn SB) set rev)" where
 "medGeneralTransition delaySet resetSet dropBehaviour (s,f) = (if sbeDom f = medInDom then 
-    Rev {(s, tsynDelay n (medOut out)) | n s out. n\<in>delaySet  \<and> (s, out)\<in>(medGeneralTransitionH resetSet dropBehaviour s (medMessageTransform ((Rep_sbElem f)\<rightharpoonup>(\<C> ''in''))))} 
-  else undefined)"
+    Rev {(sNext, tsynDelay n\<cdot>(medOut out)) | n sNext out. n\<in>delaySet  \<and> (sNext, out)\<in>(medGeneralTransitionH resetSet dropBehaviour s (medMessageTransform ((Rep_sbElem f)\<rightharpoonup>(\<C> ''in''))))} 
+  else Rev {undefined})"
 
 lift_definition medGeneralAut :: "nat set \<Rightarrow> medState set \<Rightarrow> ('a \<Rightarrow> ('a tsyn set)) \<Rightarrow> (medState, 'a medMessage tsyn) ndAutomaton" is 
   "\<lambda>delaySet resetSet dropBehaviour. (medGeneralTransition delaySet resetSet dropBehaviour, Rev {(n, medOut - )| n. n \<in> resetSet}, Discr medInDom, Discr medOutDom)"
@@ -47,23 +47,83 @@ definition medGurantee :: "medState \<Rightarrow> 'a medMessage tsyn SPS" where
 
 
 
-lemma medfairaut_dom[simp]: "ndaDom\<cdot>(medGeneralAut d r b ) = medInDom"
+lemma medgen_dom[simp]: "ndaDom\<cdot>(medGeneralAut d r b ) = medInDom"
   by (simp add: medGeneralAut.rep_eq ndaDom.rep_eq)
 
-lemma medfairaut_ran[simp]: "ndaRan\<cdot>(medGeneralAut d r b ) = medOutDom"
+lemma medgen_ran[simp]: "ndaRan\<cdot>(medGeneralAut d r b ) = medOutDom"
   by (simp add: medGeneralAut.rep_eq ndaRan.rep_eq)
 
+lemma medgen_trans[simp]: "ndaTransition\<cdot>(medGeneralAut Delay Reset Drop) = medGeneralTransition Delay Reset Drop"
+  by (simp add: medGeneralAut.rep_eq ndaTransition.rep_eq)
 
-(*
-lemma medfair_transition_tick [simp]: "medGeneralTransition (state, (medInElem -)) = Rev {(state, medOut -)}"
+lemma medgen_transh_total:  "Reset\<noteq>{} \<Longrightarrow> (\<And>m. Drop m \<noteq> {}) \<Longrightarrow>  medGeneralTransitionH Reset Drop s m \<noteq> {}"
+  apply(cases m)
+   apply(cases s)
+  by simp_all
+
+lemma medgen_trans_total_h: "Delay\<noteq>{} \<Longrightarrow> Reset\<noteq>{} \<Longrightarrow> (\<And>m. Drop m \<noteq> {}) \<Longrightarrow> medGeneralTransition Delay Reset Drop (s,sbe) \<noteq> Rev {}"
+  apply(simp)
+  apply(cases "sbeDom sbe \<noteq> medInDom")
+   apply simp
+  apply auto
+  by (metis all_not_in_conv medgen_transh_total old.prod.exhaust)
+
+lemma medgen_trans_total[simp]: "Delay\<noteq>{} \<Longrightarrow> Reset\<noteq>{} \<Longrightarrow> (\<And>m. Drop m \<noteq> {}) \<Longrightarrow> medGeneralTransition Delay Reset Drop s \<noteq> Rev {}"
+  by (metis medgen_trans_total_h surj_pair)
+
+
+lemma medgen_trans_tick [simp]: 
+    "medGeneralTransition Delay Reset Drop (state, (medInElem -)) = Rev {(state, tsynDelay n\<cdot>(medOut -)) | n::nat. n \<in> Delay}"
   by(simp add: sbeNull.rep_eq medInDom_def medInElem.simps)
 
-lemma medfair_transition_msg_suc [simp]: "medGeneralTransition (Suc n, (medInElem (Msg m))) = Rev {(n, medOut -)}"
+lemma medfair_transition_msg_suc [simp]: 
+  shows "medGeneralTransition Delay Reset Drop (Suc n, (medInElem (Msg m))) = Rev {(n, tsynDelay na\<cdot>(medOut out)) |(na::nat) out::'a tsyn. na \<in> Delay \<and> out \<in> Drop m}"
   by(simp add: medInMsgElem.rep_eq medInDom_def medInElem.simps)
 
-lemma medfair_transition_msg_0 [simp]: "medGeneralTransition (0, (medInElem (Msg m))) = Rev {(n, medOut (Msg m)) | n. True}"
-  by(auto simp add: medInMsgElem.rep_eq medInDom_def image_iff medInElem.simps)
-*)
+lemma medfair_transition_msg_0 [simp]: 
+    "medGeneralTransition Delay Reset Drop (0, (medInElem (Msg m))) = Rev {(sNext, tsynDelay n\<cdot>(medOut (\<M> m))) |(n::nat) sNext::nat. n \<in> Delay \<and> sNext \<in> Reset}"
+  by(simp add: medInMsgElem.rep_eq medInDom_def image_iff medInElem.simps)
+
+
+lemma medinelem_get_id[simp]: "(medMessageTransform Rep_sbElem (medInElem m)\<rightharpoonup>\<C> ''in'') = m"
+apply(cases m)
+  by(simp add: medInElem.simps medInMsgElem.rep_eq sbeNull.rep_eq medInDom_def)+
+
+lemma medgen_init_total[simp]: assumes "Reset\<noteq>{}" 
+  shows "ndaInitialState\<cdot>(medGeneralAut Delay Reset Drop) \<noteq> Rev {}"
+  by(simp add: ndaInitialState.rep_eq medGeneralAut.rep_eq assms)
+
+lemma med_gen_step_tick: assumes "Delay\<noteq>{}" and  "Reset\<noteq>{}" and "(\<And>m. Drop m \<noteq> {})"
+shows "spsConcIn (medIn -) (medGeneral Delay Reset Drop s) = 
+  ndaConcOutFlatten medInDom medOutDom (Rev {(s, tsynDelay n\<cdot>(medOut -)) | n::nat. n \<in> Delay}) (medGeneral Delay Reset Drop)"
+  apply(simp add: medIn_def medGeneral_def)
+  apply(subst nda_h_I)
+     apply simp_all
+   apply(rule nda_consistent)
+    apply(simp_all add: assms )
+  by (metis medGeneral_def)
+
+
+lemma med_gen_step_msg_suc: assumes "Delay\<noteq>{}" and  "Reset\<noteq>{}" and "(\<And>m. Drop m \<noteq> {})"
+shows "spsConcIn (medIn (Msg m)) (medGeneral Delay Reset Drop (Suc s)) = 
+  ndaConcOutFlatten medInDom medOutDom (Rev {(s, tsynDelay n\<cdot>(medOut out)) |(n::nat) out::'a tsyn. n \<in> Delay \<and> out \<in> Drop m}) (medGeneral Delay Reset Drop)"
+  apply(simp add: medIn_def medGeneral_def)
+  apply(subst nda_h_I)
+     apply simp_all
+   apply(rule nda_consistent)
+    apply(simp_all add: assms )
+  by (metis medGeneral_def)
+
+
+lemma med_gen_step_msg_0: assumes "Delay\<noteq>{}" and  "Reset\<noteq>{}" and "(\<And>m. Drop m \<noteq> {})"
+shows "spsConcIn (medIn (Msg m)) (medGeneral Delay Reset Drop 0) = 
+  ndaConcOutFlatten medInDom medOutDom (Rev {(sNext, tsynDelay n\<cdot>(medOut (\<M> m))) |(n::nat) sNext::nat. n \<in> Delay \<and> sNext \<in> Reset}) (medGeneral Delay Reset Drop)"
+  apply(simp add: medIn_def medGeneral_def)
+  apply(subst nda_h_I)
+     apply simp_all
+   apply(rule nda_consistent)
+    apply(simp_all add: assms )
+  by (metis medGeneral_def)
 
 
 end
